backend/Linearizeproof.v
@@ -509,18 +509,10 @@ Inductive match_states: LTL.state -> Linear.state -> Prop :=
       match_states (LTL.Block s f sp bb ls m)
                    (Linear.State ts tf sp (linearize_block bb c) ls m)
   | match_states_call:
-<<<<<<< HEAD
-      forall s vf ls m ts,
+      forall s vf ls m ts id,
       list_forall2 match_stackframes s ts ->
-      match_states (LTL.Callstate s vf ls m)
-                   (Linear.Callstate ts vf ls m)
-=======
-      forall s f ls m tf ts id,
-      list_forall2 match_stackframes s ts ->
-      transf_fundef f = OK tf ->
-      match_states (LTL.Callstate s f ls m id)
-                   (Linear.Callstate ts tf ls m id)
->>>>>>> origin/StackAware-new
+      match_states (LTL.Callstate s vf ls m id)
+                   (Linear.Callstate ts vf ls m id)
   | match_states_return:
       forall s ls m ts,
       list_forall2 match_stackframes s ts ->
@@ -665,11 +657,7 @@ Proof.
   (* internal functions *)
   assert (REACH: (reachable f)!!(LTL.fn_entrypoint f) = true).
     apply reachable_entrypoint.
-<<<<<<< HEAD
   apply functions_translated in FIND as (tf & FIND & MATCH). monadInv MATCH.
-=======
-  monadInv H9.
->>>>>>> origin/StackAware-new
   left; econstructor; split.
   apply plus_one. eapply exec_function_internal; eauto.
   rewrite (stacksize_preserved _ _ EQ). eauto.
@@ -677,12 +665,8 @@ Proof.
   econstructor; eauto. simpl. eapply is_tail_add_branch. constructor.
 
   (* external function *)
-<<<<<<< HEAD
   apply functions_translated in FIND as (tf & FIND & MATCH). monadInv MATCH.
   left; econstructor; split.
-=======
-  monadInv H9. left; econstructor; split.
->>>>>>> origin/StackAware-new
   apply plus_one. eapply exec_function_external; eauto.
   econstructor; eauto.
 
@@ -697,7 +681,6 @@ Lemma transf_initial_states q:
   forall st1, LTL.initial_state ge q st1 ->
   exists st2, Linear.initial_state tge q st2 /\ match_states st1 st2.
 Proof.
-<<<<<<< HEAD
   intros. inversion H. subst rs0.
   exploit functions_translated; eauto. intros [tf [A B]].
   pose proof (sig_preserved _ _ B) as SIG. monadInv B. cbn in SIG. rewrite <- SIG.
@@ -713,48 +696,22 @@ Lemma transf_external:
 Proof.
   intros S R q HSR Hq. destruct Hq; inv HSR.
   edestruct functions_translated as (tf & FIND & TF); eauto. monadInv TF.
-  split. econstructor; eauto. intros r S' HS'. inv HS'. rewrite H7 in H; inv H.
+  split. econstructor; eauto. intros r S' HS'. inv HS'. rewrite H8 in H; inv H.
   eexists. split; econstructor; eauto.
-=======
-  intros. inversion H.
-  exploit function_ptr_translated; eauto. intros [tf [A B]].
-  exists (Callstate nil tf (Locmap.init Vundef) m1 (prog_main tprog)); split.
-  econstructor; eauto. eapply (Genv.init_mem_transf_partial TRANSF); eauto.
-  rewrite (match_program_main TRANSF).
-  rewrite symbols_preserved. eauto.
-  rewrite <- H3. apply sig_preserved. auto.
-  rewrite (match_program_main TRANSF).
-  constructor. constructor. auto.
->>>>>>> origin/StackAware-new
 Qed.
 
 Lemma transf_final_states:
   forall st1 st2 r,
   match_states st1 st2 -> LTL.final_state st1 r -> Linear.final_state st2 r.
 Proof.
-<<<<<<< HEAD
   intros. inv H0. inv H. inv H4. inv H1. econstructor; eauto.
-=======
-  intros. inv H0. inv H. inv H5. econstructor; eauto.
-Qed.
-
-Theorem transf_program_correct:
-  forward_simulation (LTL.semantics fn_stack_requirements prog)
-                     (Linear.semantics fn_stack_requirements tprog).
-Proof.
-  eapply forward_simulation_star.
-  apply senv_preserved.
-  eexact transf_initial_states.
-  eexact transf_final_states.
-  eexact transf_step_correct.
->>>>>>> origin/StackAware-new
 Qed.
 
 End LINEARIZATION.
 
-Theorem transf_program_correct prog tprog:
+Theorem transf_program_correct prog tprog fn_stack_requirements:
   match_prog prog tprog ->
-  forward_simulation cc_id cc_id (LTL.semantics prog) (Linear.semantics tprog).
+  forward_simulation cc_id cc_id (LTL.semantics fn_stack_requirements prog) (Linear.semantics fn_stack_requirements tprog).
 Proof.
   fsim eapply forward_simulation_star; cbn in *; subst.
   - intros q _ [ ]. eapply Genv.is_internal_transf_partial_id; eauto.
